src/riot/asn1/ASN1.Low.Length.fsti
@@ -15,6 +15,8 @@ open FStar.Integers
 
 #reset-options "--fuel 0 --ifuel 0"
 
+noextract inline_for_extraction unfold
+[@@ "opaque_to_smt"]
 let len_of_asn1_length
   (len: asn1_int32)
 : (offset: size_t{v offset == Seq.length (serialize serialize_asn1_length len)})
