src/riot/asn1/ASN1.Low.Value.BigInteger.fsti
@@ -19,6 +19,8 @@ module B32 = FStar.Bytes
 let serialize32_asn1_length_of_big_integer_backwards
 : serializer32_backwards (serialize_asn1_length_of_big_integer)
 = serialize32_asn1_length_of_bound_backwards 1ul (asn1_int32_max - 6ul)
+  `coerce_serializer32_backwards _`
+  (assert_norm (bounded_int32 1 (asn1_length_max - 6) == asn1_value_int32_of_big_integer))
 
 inline_for_extraction
 val serialize32_big_integer_as_octet_string_backwards
