src/riot/asn1/ASN1.Low.Value.OID.fst
@@ -57,23 +57,23 @@ let oid_PKCS9_CSR_EXT_REQ_as_buffer        = IB.igcmalloc_of_list HS.root (oid_P
    will be marded as `noextract`.
 *)
 
-let len_of_oid oid
-= match oid with
-  | OID_RIOT                     -> 9ul
-  | OID_AT_CN                    -> 3ul
-  | OID_AT_COUNTRY               -> 3ul
-  | OID_AT_ORGANIZATION          -> 3ul
-  | OID_CLIENT_AUTH              -> 7ul
-  | OID_AUTHORITY_KEY_IDENTIFIER -> 3ul
-  | OID_KEY_USAGE                -> 3ul
-  | OID_EXTENDED_KEY_USAGE       -> 3ul
-  | OID_BASIC_CONSTRAINTS        -> 3ul
-  | OID_DIGEST_SHA256            -> 9ul
-  | OID_EC_ALG_UNRESTRICTED      -> 5ul
-  | OID_EC_GRP_SECP256R1         -> 6ul
-  | OID_ED25519                  -> 3ul
-  | OID_X25519                   -> 3ul
-  | OID_PKCS9_CSR_EXT_REQ        -> 9ul
+// let len_of_oid oid
+// = match oid with
+//   | OID_RIOT                     -> 9ul
+//   | OID_AT_CN                    -> 3ul
+//   | OID_AT_COUNTRY               -> 3ul
+//   | OID_AT_ORGANIZATION          -> 3ul
+//   | OID_CLIENT_AUTH              -> 7ul
+//   | OID_AUTHORITY_KEY_IDENTIFIER -> 3ul
+//   | OID_KEY_USAGE                -> 3ul
+//   | OID_EXTENDED_KEY_USAGE       -> 3ul
+//   | OID_BASIC_CONSTRAINTS        -> 3ul
+//   | OID_DIGEST_SHA256            -> 9ul
+//   | OID_EC_ALG_UNRESTRICTED      -> 5ul
+//   | OID_EC_GRP_SECP256R1         -> 6ul
+//   | OID_ED25519                  -> 3ul
+//   | OID_X25519                   -> 3ul
+//   | OID_PKCS9_CSR_EXT_REQ        -> 9ul
 
 (* NOTE: The order will affect Z3 for some reason. *)
 (* NOTE: Check the type of this function if a proof regression happened. *)
